Update for x86-64 model and tools.
- x64Theory now includes an instruction encoder.
- The functions in x64_stepLib have been renamed, e.g. x64_step is now x64_step_hex.

examples/l3-machine-code/x64/prog/x64_progLib.sml
@@ -265,7 +265,7 @@ in
       (* utilsLib.cache 2000 String.compare *)
          (fn s =>
              let
-                val thm = x64_stepLib.x64_step s
+                val thm = x64_stepLib.x64_step_hex s
                 val t = x64_mk_pre_post thm
              in
                 case !x64_spec_trace of
